helping/HelpingOff.v
@@ -5,7 +5,7 @@ Module HelpingOff. Section HelpingOff.
   Context `{!crisG Γ Σ α β τ _S _I, !concG}.
 
   Context (mn : string).
-  Context `{LeibnizEquiv jobID} (jobcode : jobID → itree Helping.pureE unit).
+  Context {jobID : Type} (jobcode : jobID → itree Helping.pureE unit).
 
   Definition scopes := [mn].
 
